

Exercise Nr. 6
(Deadline 30.05.2022)

1

a)

Let k_1, k_2 be kernel functions with

$$\phi_1 : X \rightarrow H_1, \phi_2 : X \rightarrow H_2$$

$$k_1(x, y) = \langle \Phi_1(x), \Phi_1(y) \rangle$$

$$k_2(x, y) = \langle \Phi_2(x), \Phi_2(y) \rangle$$

$$k(x, y) = \alpha_1 k_1 + k_2$$

$$= \alpha_1 k_1(x, y) + k_2(x, y)$$

$$= \alpha_1 \langle \Phi_1(x), \Phi_1(y) \rangle + \langle \Phi_2(x), \Phi_2(y) \rangle$$

$$= \langle \alpha_1 \Phi_1(x), \Phi_1(y) \rangle + \langle \Phi_2(x), \Phi_2(y) \rangle$$

$$= \langle \alpha_1 \Phi_1(x) + \Phi_2(x), \Phi_1(y) + \Phi_2(y) \rangle$$

$$= \alpha_1 \langle \Phi_1(x) + \Phi_2(x), \Phi_1(y) + \Phi_2(y) \rangle$$

Let $\phi_3 : X \rightarrow H_3$ be a Hilbert space with

$$H_3 = H_1 \cup H_2, \Phi_3(x) = \Phi_1(x) \cup \Phi_2(x)$$

$$= \alpha_1 \langle \Phi_3(x), \Phi_3(y) \rangle$$

$$\text{Defining } k' = \langle \Phi_3(x), \Phi_3(y) \rangle$$

Let K' be the kernel matrix of k' :

$$\Rightarrow c^T K' c \leq 0 \forall c$$

$$\Rightarrow \alpha_1 c^T K' c = c^T \alpha_1 K' c \leq 0 \forall c$$

$$\Rightarrow \alpha_1 K' = K \text{ is the kernel matrix of } k$$

$$\Rightarrow k \text{ is kernel}$$

b)

Proof by counterexample: Let $k_1(x, y) = x^T y, k_2(x, y) = 2x^T y$

$$k = k_1(x, y) - k_2(x, y) = -x^T y \Rightarrow \text{not psd}$$

\Rightarrow Therefore k is not a valid kernel

c)

1. Proof: $k = k_1 * k_2$ is a kernel with k_1, k_2 being any kernels

Let k_1, k_2 be kernel functions with

$$\phi_1 : X \rightarrow H_1, \phi_2 : X \rightarrow H_2$$

$$k_1(x, y) = \langle \Phi_1(x), \Phi_1(y) \rangle$$

$$k_2(x, y) = \langle \Phi_2(x), \Phi_2(y) \rangle$$

$$k = k_1 \cdot k_2$$

$$= \langle \Phi_1(x), \Phi_1(y) \rangle \cdot \langle \Phi_2(x), \Phi_2(y) \rangle$$

$$= \sum_i (\Phi_1)_i(x) \cdot (\Phi_1)_i(y) \cdot \sum_j (\Phi_2)_j(x) \cdot (\Phi_2)_j(y)$$

$$= \sum_i \sum_j (\Phi_1)_i(x) \cdot (\Phi_1)_i(y) \cdot (\Phi_2)_j(x) \cdot (\Phi_2)_j(y)$$

$$= \sum_i \sum_j (\Phi_1)_i(x) \cdot (\Phi_2)_j(x) \cdot (\Phi_1)_i(y) \cdot (\Phi_2)_j(y)$$

$$= \sum_i \sum_j (\Phi_3)_{ij}(x) \cdot (\Phi_3)_{ij}(y)$$

$$= \langle \Phi_3(x), \Phi_3(y) \rangle$$

$$\text{With } \phi_3 : X \rightarrow H_3 : (\Phi_3)_{ij}(x) = (\Phi_1)_i(x) \cdot (\Phi_2)_j(x)$$

$$H_3 = H_1 \times H_2 \text{ is a Hilbert space, the norm is given by: } \|(x, y)\| = \sqrt{\|x\|_{H_1}^2 + \|y\|_{H_2}^2}$$

$$\implies k \text{ is kernel}$$

2. Proof: $\bar{k} = f(x)f(y)$ is a kernel with $f(x), f(y)$ being any functions

$$\bar{k} = f(x)f(y) = \langle f(x), f(y) \rangle$$

if f is one-dimensional, \bar{k} is a kernel as well. From above we know that the multiplication of two kernels is a kernel as well. Therefore $k = f(x) * k_1(x, y) * f(y) = k_1(x, y) * f(x)f(y) = k_1 * \bar{k}$ is a kernel.

d)

$$\begin{aligned} k(x, y) &= \frac{k_1(x, y)}{\sqrt{k_1(x, x)k_2(y, y)}} \\ &= \frac{1}{\sqrt{k_1(x, x)}} k_1(x, y) \frac{1}{\sqrt{k_1(y, y)}} \\ &= f(x) k_1(x, y) f(y) \end{aligned}$$

$$\text{with } f(x) = \frac{1}{\sqrt{k_1(x, x)}}$$

$$f(y) = \frac{1}{\sqrt{k_1(y, y)}}$$

see c) for the proof that a k of this form is a kernel

2

\Rightarrow next weeks assignment

3

a)

The setting can be applied to friendship connections within communities or to the traveling salesman problem with different locations on a map.

b)

$$\begin{aligned}
 f^T L f &= \sum_{i,j} f_i f_j L_{ij} \\
 &= \sum_{i,j} f_i f_j (D_{ij} - A_{ij}) \\
 &= \sum_{i,j} f_i f_j D_{ij} - \sum_{i,j} f_i f_j A_{ij} \\
 &= \sum_i D_{ii} f_i^2 - \sum_{i \sim j} f_i f_j \\
 &= \frac{1}{2} \sum_i D_{ii} f_i^2 - \sum_{i \sim j} f_i f_j + \frac{1}{2} \sum_j D_{jj} f_j^2 \\
 &= \left(\frac{1}{2} \sum_i \left[\sum_{j \text{ with: } i \sim j} f_i^2 \right] - \sum_{i \sim j} f_i f_j + \frac{1}{2} \sum_j \left[\sum_{i \text{ with: } i \sim j} f_j^2 \right] \right) \\
 &= \frac{1}{2} \sum_{i \sim j} f_i^2 - \sum_{i \sim j} f_i f_j + \frac{1}{2} \sum_{i \sim j} f_j^2 \\
 &= \frac{1}{2} \sum_{i \sim j} (f_i^2 - 2f_i f_j + f_j^2) \\
 &= \frac{1}{2} \sum_{i \sim j} (f_i - f_j)^2 \\
 &= \Omega(f)^2
 \end{aligned}$$

c)

Well Defined

$$f, g \in \mathcal{H} \implies f, g \in \mathbb{R}^n$$

thus, they are unique and $\langle f, g \rangle_{\mathcal{H}} = f^T L g$ is well-defined

Linearity

show:

$$\langle x_1 + x_2, y \rangle = \langle x_1, y \rangle + \langle x_2, y \rangle$$

$$\begin{aligned} \langle f_1 + f_2, g \rangle_{\mathcal{H}} &= (f_1 + f_2)^T Lg \\ &= \sum_{ij} (f_{1i} + f_{2i}) L_{ij} g_j \\ &= \sum_{ij} f_{1i} L_{ij} g_j + \sum_{ij} f_{2i} L_{ij} g_j \\ &= f_1^T Lg + f_2^T Lg \\ &= \langle f_1, g \rangle_{\mathcal{H}} + \langle f_2, g \rangle_{\mathcal{H}} \end{aligned}$$

show:

$$\langle \lambda x, y \rangle = \lambda \langle x, y \rangle \quad \forall \lambda \in \mathbb{R}$$

$$\begin{aligned} \langle \lambda f, g \rangle_{\mathcal{H}} &= (\lambda f^T) Lg \\ &= \lambda (f^T Lg) \\ &= \lambda \langle f, g \rangle_{\mathcal{H}} \end{aligned}$$

Symmetry

show:

$$\langle x, y \rangle = \langle y, x \rangle$$

$$\begin{aligned} \langle f, g \rangle_{\mathcal{H}} &= f^T Lg \\ &= \sum_{ij} f_i L_{ij} g_j \\ &= \sum_{ij} g_j L_{ij} f_i \\ &= g^T Lf \\ &= \langle g, f \rangle_{\mathcal{H}} \end{aligned}$$

Pos. Def.

show:

$$\langle x, x \rangle \geq 0$$

$$\begin{aligned} \langle f, f \rangle_{\mathcal{H}} &= f^T Lf \\ &= \Omega(f)^2 \geq 0 \end{aligned}$$

show:

$$\langle x, x \rangle = 0 \implies x = 0$$

$$\langle f, f \rangle_{\mathcal{H}} = 0$$

$$\implies \Omega(f)^2 = 0$$

$$\implies \sum_{i \sim j} (f_i - f_j)^2 = 0$$

$$\implies f_i = f_j \quad \forall i, j : i \sim j$$

as graph is connected:

$$\implies f_i = f_j \quad \forall i, j$$

$$\text{as } \sum_{i=1}^n f_i = 0 :$$

$$\implies f_i = 0 \quad \forall i$$

$$\iff f = 0$$

$\implies \langle f, g \rangle_{\mathcal{H}}$ is a scalar product on \mathcal{H}

d)

Let $k(i, j) \in \mathbb{R}$ be the weight of the edge between the nodes i and j
Then $\Phi(i)$ is the vector of edge weights to all other nodes.